Make action_graph type more abstract; proofs feel cleaner and clearer.

hol/datadepsScript.sml
@@ -1,6 +1,7 @@
 open HolKernel Parse boolLib bossLib;
 open primitivesTheory forLoopTheory pred_setTheory
 open listRangeTheory
+open listTheory
 open lcsymtacs
 
 fun asimp thl = asm_simp_tac (srw_ss() ++ ARITH_ss) thl
@@ -69,34 +70,81 @@ val touches_SYM = store_thm(
   ``touches a1 a2 ⇒ touches a2 a1``,
   simp[touches_def] >> rpt strip_tac >> simp[]);
 
-val _ = type_abbrev ("action_graph",
-                     ``:'a action set # ('a action -> 'a action -> bool)``);
+val _ = Hol_datatype`action_graph = <| nodes : 'a action set;
+                                       edges : 'a action -> 'a action set |>`
+
+val _ = overload_on ("IN", ``λa:'a action G:'a action_graph. a ∈ G.nodes``)
+
+val graph_equality = store_thm(
+  "graph_equality",
+  ``G1 = G2 ⇔
+      (∀a. a ∈ G1 ⇔ a ∈ G2) ∧ (∀a1 a2. G1.edges a1 a2 ⇔ G2.edges a1 a2)``,
+  simp[theorem "action_graph_component_equality", Once EQ_IMP_THM] >>
+  strip_tac >> conj_tac >- simp[EXTENSION] >> simp[FUN_EQ_THM]);
 
 val wfG_def = Define`
-  wfG (els,R) ⇔
-      FINITE els ∧
-      (∀a1 a2. R a1 a2 ⇒ touches a1 a2 ∧ a1 ∈ els ∧ a2 ∈ els) ∧
-      (∀a1 a2. a1 ∈ els ∧ a2 ∈ els ∧ touches a1 a2 ∧ a1 ≠ a2 ⇒ (¬R a1 a2 ⇔ R a2 a1)) ∧
-      ∀a1 a2. a1 ∈ els ∧ a2 ∈ els ∧ R⁺ a1 a2 ⇒ ¬R⁺ a2 a1
+  wfG G ⇔
+      FINITE G.nodes ∧
+      (∀a1 a2. G.edges a1 a2 ⇒ touches a1 a2 ∧ a1 ∈ G ∧ a2 ∈ G) ∧
+      (∀a1 a2. a1 ∈ G ∧ a2 ∈ G ∧ touches a1 a2 ∧ a1 ≠ a2 ⇒ (¬G.edges a1 a2 ⇔ G.edges a2 a1)) ∧
+      ∀a1 a2. a1 ∈ G ∧ a2 ∈ G ∧ G.edges⁺ a1 a2 ⇒ ¬G.edges⁺ a2 a1
 `;
+
+val emptyG_def = Define`
+  emptyG = <| nodes := ∅; edges := REMPTY |>
+`;
+
+val IN_emptyG = store_thm(
+  "IN_emptyG",
+  ``a ∈ emptyG ⇔ F``,
+  simp[emptyG_def]);
+val _ = export_rewrites ["IN_emptyG"]
+
+val emptyG_edges = store_thm(
+  "emptyG_edges",
+  ``emptyG.edges x y ⇔ F``,
+  simp[emptyG_def]);
+val _ = export_rewrites ["emptyG_edges"]
 
 val wfG_empty = store_thm(
   "wfG_empty",
-  ``wfG (∅, REMPTY)``,
-  simp[wfG_def]);
+  ``wfG emptyG``,
+  simp[wfG_def, emptyG_def]);
 val _ = export_rewrites ["wfG_empty"]
 
 val wfG_irrefl = store_thm(
   "wfG_irrefl",
-  ``wfG (es,R) ∧ x ∈ es ⇒ ¬R x x``,
+  ``wfG G ∧ x ∈ G ⇒ ¬G.edges x x``,
   simp[wfG_def] >> rpt strip_tac >>
   metis_tac[relationTheory.TC_SUBSET]);
 
+val gDELETE_def = Define`
+  gDELETE G a = <| nodes := G.nodes DELETE a; edges := G.edges \\ a |>
+`;
+val _ = overload_on ("\\\\", ``gDELETE``)
+
+val IN_gDELETE = store_thm(
+  "IN_gDELETE",
+  ``a ∈ G \\ b ⇔ a ∈ G ∧ a ≠ b``,
+  simp[gDELETE_def]);
+val _ = export_rewrites ["IN_gDELETE"]
+
+val gDELETE_edges = store_thm(
+  "gDELETE_edges",
+  ``(G \\ a).edges b c ⇔ G.edges b c ∧ a ≠ b``,
+  simp[gDELETE_def] >> metis_tac[]);
+val _ = export_rewrites ["gDELETE_edges"]
+
+val gDELETE_commutes = store_thm(
+  "gDELETE_commutes",
+  ``(G:'a action_graph) \\ a1 \\ a2 = G \\ a2 \\ a1``,
+  simp[gDELETE_def, theorem "action_graph_component_equality", DELETE_COMM] >>
+  simp[FUN_EQ_THM] >> metis_tac[]);
+
 val wfGs_pull_apart = store_thm(
   "wfGs_pull_apart",
-  ``wfG (a INSERT as, R) ∧ (∀a'. a' ∈ as ⇒ ¬R a' a) ∧ a ∉ as ⇒
-    wfG (as, R \\ a)``,
-  simp[wfG_def] >> rw[] >>
+  ``wfG G ∧ a ∈ G ∧ (∀a'. a' ∈ G ⇒ ¬G.edges a' a) ⇒ wfG (G \\ a)``,
+  simp[wfG_def, gDELETE_def] >> rw[] >>
   metis_tac[relationTheory.TC_MONOTONE, relationTheory.RDOM_DELETE_DEF]);
 
 val _ = IndDefLib.export_rule_induction "relation.TC_STRONG_INDUCT"
@@ -107,9 +155,9 @@ val TC_in_R = store_thm(
 
 val wfG_WF = store_thm(
   "wfG_WF",
-  ``wfG (es, R) ⇒ WF R``,
+  ``wfG G ⇒ WF G.edges``,
   simp[wfG_def] >> strip_tac >>
-  `R = REL_RESTRICT R es`
+  `G.edges = REL_RESTRICT G.edges G.nodes`
     by (simp[REL_RESTRICT_DEF, FUN_EQ_THM, EQ_IMP_THM] >>
         metis_tac[]) >>
   first_assum (fn th => simp[FINITE_WF_noloops, Once th]) >>
@@ -118,31 +166,31 @@ val wfG_WF = store_thm(
 
 val wfG_FINITE = store_thm(
   "wfG_FINITE",
-  ``wfG (es,R) ⇒ FINITE es``,
+  ``wfG G ⇒ FINITE G.nodes``,
   simp[wfG_def]);
 
 val nonempty_wfG_has_points = store_thm(
   "nonempty_wfG_has_points",
-  ``wfG (es, R) ∧ es ≠ ∅ ⇒
-    ∃e. e ∈ es ∧ ∀e'. e' ∈ es ⇒ ¬R e' e``,
+  ``wfG G ∧ G.nodes ≠ ∅ ⇒
+    ∃e. e ∈ G ∧ ∀e'. e' ∈ G ⇒ ¬G.edges e' e``,
   rpt strip_tac >>
-  `WF R` suffices_by
+  `WF G.edges` suffices_by
     (simp[relationTheory.WF_DEF, IN_DEF] >>
      pop_assum mp_tac >> simp[GSYM MEMBER_NOT_EMPTY, IN_DEF] >>
      metis_tac[]) >>
   metis_tac[wfG_WF]);
 
 val (evalG_rules,evalG_ind,evalG_cases) = Hol_reln`
-  (∀A R. evalG A (∅, R) A) ∧
-  (∀a as A0 A R.
-      (∀a'. a' ∈ as ⇒ ¬R a' a) ∧ a ∉ as ∧
-      evalG (apply_action a A0) (as, R \\ a) A ⇒
-      evalG A0 (a INSERT as, R) A)
+  (∀A. evalG A emptyG A) ∧
+  (∀a A0 G A.
+      a ∈ G ∧ (∀a'. a' ∈ G ⇒ ¬G.edges a' a) ∧
+      evalG (apply_action a A0) (G \\ a) A ⇒
+      evalG A0 G A)
 `;
 
 val evalG_EMPTY = store_thm(
   "evalG_EMPTY",
-  ``evalG A0 (∅, R) A ⇔ A = A0``,
+  ``evalG A0 emptyG A ⇔ A = A0``,
   simp[Once evalG_cases]);
 val _ = export_rewrites ["evalG_EMPTY"]
 
@@ -151,100 +199,80 @@ val INSERT_11 = store_thm(
   ``e ∉ s1 ∧ e ∉ s2 ⇒ (e INSERT s1 = e INSERT s2 ⇔ s1 = s2)``,
   simp[EQ_IMP_THM] >> simp[EXTENSION] >> metis_tac[]);
 
+val _ = overload_on ("gCARD", ``\g. CARD g.nodes``)
+
+val gCARD_EQ_0 = store_thm(
+  "gCARD_EQ_0",
+  ``wfG G ⇒ (gCARD G = 0 ⇔ G = emptyG)``,
+  simp[emptyG_def, wfG_def, EQ_IMP_THM] >> rpt strip_tac >> fs[] >>
+  simp[theorem "action_graph_component_equality", FUN_EQ_THM]);
+
+val gCARD_gDELETE = store_thm(
+  "gCARD_gDELETE",
+  ``wfG G ∧ a ∈ G ⇒ gCARD (G \\ a) = gCARD G - 1``,
+  simp[wfG_def, gDELETE_def]);
+val _ = export_rewrites ["gCARD_gDELETE"]
+
 val evalG_total = store_thm(
   "evalG_total",
   ``wfG G ⇒ ∃A'. evalG A G A'``,
-  pairLib.PairCases_on `G` >> map_every qabbrev_tac [`es = G0`, `R = G1`] >>
-  markerLib.RM_ALL_ABBREVS_TAC >>
-  map_every qid_spec_tac [`A`, `R`] >>
-  Induct_on `CARD es`
-  >- (simp[Once evalG_cases] >> metis_tac[CARD_EQ_0, wfG_def]) >>
-  qx_gen_tac `es` >> strip_tac >>
-  `es ≠ ∅` by (strip_tac >> fs[]) >>
-  map_every qx_gen_tac [`R`, `A0`] >> strip_tac >>
-  `∃e. e ∈ es ∧ ∀e'. e' ∈ es ⇒ ¬R e' e` by metis_tac[nonempty_wfG_has_points] >>
-  `∃es0. e ∉ es0 ∧ es = e INSERT es0` by metis_tac[DECOMPOSITION] >>
-  `FINITE es` by fs[wfG_def] >> rw[] >> fs[] >>
-  first_x_assum (qspec_then `es0` mp_tac) >> simp[] >>
-  disch_then (qspecl_then [`R \\ e`, `apply_action e A0`] mp_tac) >>
-  `wfG (es0, R \\ e)` by metis_tac[wfGs_pull_apart] >> simp[] >>
-  disch_then (qx_choose_then `A0'` assume_tac) >>
+  qid_spec_tac `A` >> Induct_on `gCARD G`
+  >- (simp[Once evalG_cases] >> metis_tac[gCARD_EQ_0]) >>
+  rpt strip_tac >>
+  `G.nodes ≠ ∅` by (strip_tac >> fs[]) >>
+  `∃a. a ∈ G ∧ ∀a'. a' ∈ G ⇒ ¬G.edges a' a`
+    by metis_tac[nonempty_wfG_has_points] >>
+  `wfG (G \\ a)` by metis_tac[wfGs_pull_apart] >>
+  `gCARD (G \\ a) = v` by simp[] >>
   metis_tac[evalG_rules]);
 
 val wfG_evaluate_deterministically = store_thm(
   "wfG_evaluate_deterministically",
-  ``wfG G ∧ evalG A0 G A ⇒
-    ∀A'. evalG A0 G A' ⇒ A' = A``,
-  pairLib.PairCases_on `G` >> map_every qabbrev_tac [`es = G0`, `R = G1`] >>
-  markerLib.RM_ALL_ABBREVS_TAC >>
-  map_every qid_spec_tac [`A0`, `A`, `R`] >>
-  completeInduct_on `CARD es` >>
-  qx_gen_tac `es` >>
-  qmatch_rename_tac `n = CARD es ⇒ XX` ["XX"] >> strip_tac >>
-  map_every qx_gen_tac [`R`, `A`, `A0`] >> strip_tac >>
+  ``wfG G ∧ evalG A0 G A ⇒ ∀A'. evalG A0 G A' ⇒ A' = A``,
+  map_every qid_spec_tac [`A0`, `A`] >>
+  completeInduct_on `gCARD G` >> qx_gen_tac `G` >>
+  qmatch_rename_tac `n = gCARD G ⇒ XX` ["XX"] >> strip_tac >>
+  map_every qx_gen_tac [`A`, `A0`] >> strip_tac >>
   qx_gen_tac `A'` >> strip_tac >>
   full_simp_tac (srw_ss() ++ boolSimps.DNF_ss)
     [AND_IMP_INTRO, GSYM CONJ_ASSOC] >> rw[] >>
-  qpat_assum `evalG A0 (es, R) A` mp_tac >>
+  qpat_assum `evalG A0 G A` mp_tac >>
   simp[Once evalG_cases] >>
   disch_then (DISJ_CASES_THEN2
                 strip_assume_tac
-                (qx_choosel_then [`e1`, `es1`] strip_assume_tac))
+                (qx_choose_then `a1` strip_assume_tac))
   >- fs[] >>
+  `G ≠ emptyG` by (strip_tac >> fs[]) >>
   qpat_assum `evalG XX YY A'` mp_tac >>
   simp[Once evalG_cases] >>
-  disch_then (qx_choosel_then [`e2`, `es2`] strip_assume_tac) >>
-  Cases_on `e2 = e1`
-  >- (rw[] >>
-      `es2 = es1` by metis_tac[INSERT_11] >>
-      rw[] >>
-      `FINITE es1` suffices_by
-        (strip_tac >> fs[] >>
-         metis_tac[DECIDE ``x < SUC x``, wfGs_pull_apart]) >>
-      fs[wfG_def]) >>
-  `e1 ∈ es2 ∧ e2 ∈ es1` by metis_tac[EXTENSION, IN_INSERT] >>
-  `∃es0. es1 = e2 INSERT es0 ∧ es2 = e1 INSERT es0 ∧ e1 ∉ es0 ∧ e2 ∉ es0`
-    by (`∃es0. es1 = e2 INSERT es0 ∧ e2 ∉ es0` by metis_tac[DECOMPOSITION] >>
-        qexists_tac `es0` >> simp[] >> fs[] >>
-        qpat_assum `XX INSERT YY INSERT ZZ = UU INSERT VV` mp_tac >>
-        ONCE_REWRITE_TAC [INSERT_COMM] >> simp[INSERT_11]) >>
-  rw[] >>
-  `wfG (e2 INSERT es0, R \\ e1) ∧ wfG (es0, R \\ e2 \\ e1) ∧
-   wfG (e1 INSERT es0, R \\ e2) ∧ wfG (es0, R \\ e1 \\ e2)`
-    by metis_tac[wfGs_pull_apart, IN_INSERT, relationTheory.RDOM_DELETE_DEF] >>
-  `FINITE es0` by metis_tac[wfG_FINITE] >>
-  `(∃A21. evalG (apply_action e1 (apply_action e2 A0)) (es0, R \\ e2 \\ e1) A21) ∧
-   ∃A12. evalG (apply_action e2 (apply_action e1 A0)) (es0, R \\ e1 \\ e2) A12`
+  disch_then (qx_choose_then `a2` strip_assume_tac) >>
+  `wfG (G \\ a1) ∧ wfG (G \\ a2)` by simp[wfGs_pull_apart] >>
+  Cases_on `a2 = a1`
+  >- (rw[] >> first_x_assum (qspecl_then [`G \\ a1`, `A'`] match_mp_tac) >>
+      qexists_tac `apply_action a1 A0` >> simp[] >>
+      metis_tac[IN_emptyG, gCARD_EQ_0, DECIDE ``¬(0 < x) ⇔ x = 0``]) >>
+  `apply_action a1 (apply_action a2 A0) = apply_action a2 (apply_action a1 A0)`
+    by (match_mp_tac nontouching_actions_commute >> metis_tac [wfG_def]) >>
+  `wfG (G \\ a1 \\ a2)` by simp[wfGs_pull_apart] >>
+  `∃A2. evalG (apply_action a1 (apply_action a2 A0)) (G \\ a1 \\ a2) A2`
     by metis_tac[evalG_total] >>
-  `evalG (apply_action e2 A0) (e1 INSERT es0, R \\ e2) A21 ∧
-   evalG (apply_action e1 A0) (e2 INSERT es0, R \\ e1) A12`
-    by metis_tac[evalG_rules, IN_INSERT, relationTheory.RDOM_DELETE_DEF] >>
-  `A' = A21 ∧ A = A12`
-    by (conj_tac >>
-        first_x_assum match_mp_tac >| [
-          qexists_tac `e1 INSERT es0`,
-          qexists_tac `e2 INSERT es0`
-        ]>> simp[] >> metis_tac[]) >>
-  ntac 2 (pop_assum SUBST_ALL_TAC) >>
-  `R \\ e2 \\ e1 = R \\ e1 \\ e2`
-    by (simp[FUN_EQ_THM, relationTheory.RDOM_DELETE_DEF] >> metis_tac[]) >>
-  pop_assum SUBST_ALL_TAC >>
-  `apply_action e1 (apply_action e2 A0) = apply_action e2 (apply_action e1 A0)`
-    suffices_by (disch_then SUBST_ALL_TAC >> first_x_assum match_mp_tac >>
-                 qexists_tac `es0` >> simp[] >> metis_tac[]) >>
-  `¬R e2 e1 ∧ ¬R e1 e2` by metis_tac[] >>
-  `¬touches e1 e2`
-    by (qpat_assum `wfG (e1 INSERT e2 INSERT es0, R)` mp_tac >>
-        simp[wfG_def] >> metis_tac[]) >>
-  match_mp_tac nontouching_actions_commute >> simp[]);
+  `evalG (apply_action a1 A0) (G \\ a1) A2 ∧
+   evalG (apply_action a2 A0) (G \\ a2) A2`
+    by (conj_tac >> match_mp_tac (CONJUNCT2 evalG_rules) >| [
+          qexists_tac `a2`, qexists_tac `a1`] >> simp[] >>
+        metis_tac[gDELETE_commutes]) >>
+  `gCARD (G \\ a1) < gCARD G ∧ gCARD (G \\ a2) < gCARD G` suffices_by
+     metis_tac[] >>
+  simp[] >>
+  metis_tac [gCARD_EQ_0, IN_emptyG, DECIDE ``¬(0 < x) ⇔ x = 0``])
 
 val add_action_def = Define`
-  add_action a (As,R) =
-    if a ∈ As then (As,R)
+  add_action a G =
+    if a ∈ G then G
     else
-      (a INSERT As,
-       (λsrc tgt. R src tgt ∨
-                  src = a ∧ touches a tgt ∧ tgt ∈ As))
+      <| nodes := a INSERT G.nodes ;
+         edges := (λsrc tgt. G.edges src tgt ∨
+                             src = a ∧ touches a tgt ∧ tgt ∈ G.nodes) |>
 `;
 
 val add_action_lemma = prove(
@@ -259,17 +287,15 @@ val add_action_lemma = prove(
 val wfG_add_action = store_thm(
   "wfG_add_action",
   ``wfG G ⇒ wfG (add_action a G)``,
-  Cases_on `G` >>
-  qmatch_rename_tac `XX ⇒ wfG (add_action a (As,R))` ["XX"] >>
   simp[add_action_def] >>
   qabbrev_tac
-    `R' = (λsrc tgt. R src tgt ∨ src = a ∧ touches a tgt ∧ tgt ∈ As)`>>
-  Cases_on `a ∈ As` >> simp[] >>
-  `∀a1 a2. R a1 a2 ∨ a1 = a ∧ touches a a2 ∧ a2 ∈ As ⇔ R' a1 a2` by simp[Abbr`R'`] >>
+    `R' = (λsrc tgt. G.edges src tgt ∨ src = a ∧ touches a tgt ∧ tgt ∈ G)`>>
+  Cases_on `a ∈ G` >> simp[] >>
+  `∀a1 a2. G.edges a1 a2 ∨ a1 = a ∧ touches a a2 ∧ a2 ∈ G ⇔ R' a1 a2` by simp[Abbr`R'`] >>
   markerLib.RM_ALL_ABBREVS_TAC >>
   simp[wfG_def] >> reverse (rpt strip_tac)
-  >- (`∀b. ¬R a b ∧ ¬R b a` by metis_tac[] >>
-      `∀a1 a2. R' a1 a2 ⇒ R a1 a2 ∨ a1 = a ∧ a2 ≠ a` by metis_tac[] >>
+  >- (`∀b. ¬G.edges a b ∧ ¬G.edges b a` by metis_tac[] >>
+      `∀a1 a2. R' a1 a2 ⇒ G.edges a1 a2 ∨ a1 = a ∧ a2 ≠ a` by metis_tac[] >>
       pop_assum
         (fn c1 => pop_assum
            (fn c2 => assume_tac (MATCH_MP add_action_lemma (CONJ c1 c2)))) >>
@@ -287,14 +313,14 @@ val loop_to_graph_def = tDefine "loop_to_graph" `
     if lo < hi then
       add_action (mkEAction wf rfs body lo)
                  (loop_to_graph (lo+1,hi) wf rfs body)
-    else (∅, REMPTY)
+    else emptyG
 ` (WF_REL_TAC `measure (λp. SND (FST p) - FST (FST p))`)
 
 val loop_to_graph_FOLDR = store_thm(
   "loop_to_graph_FOLDR",
   ``loop_to_graph (lo,hi) wf rfs body =
       FOLDR (add_action o mkEAction wf rfs body)
-            (∅, REMPTY)
+            emptyG
             [lo ..< hi]``,
   Induct_on `hi - lo` >>
   asimp[Once loop_to_graph_def,listRangeLHI_EMPTY, listRangeLHI_CONS]);
@@ -313,28 +339,19 @@ val eval_apply_action = store_thm(
   rpt (AP_TERM_TAC ORELSE AP_THM_TAC) >> Induct_on `rfs` >>
   simp[listTheory.LIST_APPLY_DEF]);
 
-val evalG_I = store_thm(
-  "evalG_I",
-  ``∀A0 A G a As R.
-       G = (a INSERT As,R) ∧ (∀a'. a' ∈ As ⇒ ¬R a' a) ∧ a ∉ As ∧
-       evalG (apply_action a A0) (As, R \\ a) A ⇒
-       evalG A0 G A``,
-  simp[CONJUNCT2 evalG_rules]);
-
 val loop_to_graph_iterations = store_thm(
   "loop_to_graph_iterations",
-  ``loop_to_graph (lo,hi) wf rfs body = (As, R) ⇒
-      (∀a. a ∈ As ⇒ lo ≤ a.iter ∧ a.iter < hi) ∧
-      (∀a1 a2. R a1 a2 ⇒ a1 ∈ As ∧ a2 ∈ As)``,
-  map_every qid_spec_tac [`As`, `R`] >>
-  Induct_on `hi - lo` >> simp[Once loop_to_graph_def] >>
+  ``loop_to_graph (lo,hi) wf rfs body = G ⇒
+      (∀a. a ∈ G ⇒ lo ≤ a.iter ∧ a.iter < hi) ∧
+      (∀a1 a2. G.edges a1 a2 ⇒ a1 ∈ G ∧ a2 ∈ G)``,
+  qid_spec_tac `G` >> Induct_on `hi - lo` >>
+  ONCE_REWRITE_TAC [loop_to_graph_def] >- simp[] >>
   rpt gen_tac >> qmatch_rename_tac `SUC n = hi - lo ⇒ XX` ["XX"] >>
-  disch_then (assume_tac o SYM) >> map_every qx_gen_tac [`R`, `As`] >>
-  `∃As0 R0. loop_to_graph (lo + 1, hi) wf rfs body = (As0, R0)`
-    by metis_tac[TypeBase.nchotomy_of ``:'a # 'b``] >>
+  disch_then (assume_tac o SYM) >> qx_gen_tac `G` >> simp[] >>
+  `∃G0. loop_to_graph (lo + 1, hi) wf rfs body = G0` by simp[] >>
   `n = hi - (lo + 1)` by decide_tac >>
-  `(∀a. a ∈ As0 ⇒ lo + 1 ≤ a.iter ∧ a.iter < hi) ∧
-   ∀a1 a2. R0 a1 a2 ⇒ a1 ∈ As0 ∧ a2 ∈ As0` by metis_tac[] >>
+  `(∀a. a ∈ G0 ⇒ lo + 1 ≤ a.iter ∧ a.iter < hi) ∧
+   ∀a1 a2. G0.edges a1 a2 ⇒ a1 ∈ G0 ∧ a2 ∈ G0` by metis_tac[] >>
   simp[add_action_def] >> rw[] >> fs[mkEAction_def]
   >- (res_tac >> decide_tac)
   >- res_tac
@@ -354,74 +371,99 @@ val loop_to_graph_correct = store_thm(
   qmatch_rename_tac `SUC n = hi - lo ⇒ XX` ["XX"] >>
   disch_then (assume_tac o SYM) >> qx_gen_tac `A` >>
   simp[Once FOR_def, Once loop_to_graph_def, eval_apply_action] >>
-  match_mp_tac evalG_I >>
-  `∃As R0. loop_to_graph (lo + 1, hi) wf rfs body = (As,R0)`
-    by metis_tac[TypeBase.nchotomy_of ``:'a # 'b``] >>
+  match_mp_tac (CONJUNCT2 evalG_rules) >>
+  `∃G. loop_to_graph (lo + 1, hi) wf rfs body = G` by simp[] >>
   simp[add_action_def] >>
-  `mkEAction wf rfs body lo ∉ As`
+  `¬(mkEAction wf rfs body lo ∈ G)`
     by (strip_tac >>
         `lo + 1 ≤ (mkEAction wf rfs body lo).iter`
           by metis_tac[loop_to_graph_iterations] >>
         full_simp_tac (srw_ss() ++ ARITH_ss) [mkEAction_def]) >>
-  map_every qexists_tac [`mkEAction wf rfs body lo`, `As`] >>
+  qexists_tac `mkEAction wf rfs body lo` >>
   simp[] >> csimp[] >>
-  `(∀a. a ∈ As ⇒ lo + 1 ≤ a.iter ∧ a.iter < hi) ∧
-   ∀a1 a2. R0 a1 a2 ⇒ a1 ∈ As ∧ a2 ∈ As`
+  `(∀a. a ∈ G ⇒ lo + 1 ≤ a.iter ∧ a.iter < hi) ∧
+   ∀a1 a2. G.edges a1 a2 ⇒ a1 ∈ G ∧ a2 ∈ G`
     by metis_tac[loop_to_graph_iterations] >>
   `(mkEAction wf rfs body lo).iter = lo ∧ ¬(lo + 1 ≤ lo)`
     by simp[mkEAction_def] >>
   conj_tac >- metis_tac[] >>
   qmatch_abbrev_tac `
-    evalG AA (As, RR \\ act) (FOR (lo + 1, hi) (eval wf rfs body) AA)
+    evalG AA GG (FOR (lo + 1, hi) (eval wf rfs body) AA)
   ` >>
   `n = hi - (lo + 1)` by decide_tac >>
-  `RR \\ act = R0` suffices_by metis_tac[] >>
-  qunabbrev_tac `RR` >> csimp[FUN_EQ_THM] >> metis_tac[]);
+  `GG = G` suffices_by metis_tac[] >>
+  qunabbrev_tac `GG` >>
+  simp[theorem "action_graph_component_equality"] >>
+  conj_tac >- (csimp[EXTENSION] >> metis_tac[]) >>
+  csimp[FUN_EQ_THM] >> metis_tac[]);
 
 val RIMAGE_DEF = new_definition(
   "RIMAGE_DEF",
   ``RIMAGE f R x y <=> ?a b. (x = f a) /\ (y = f b) /\ R a b``);
 
+val RIMAGE_REMPTY = store_thm(
+  "RIMAGE_REMPTY",
+  ``RIMAGE f REMPTY = REMPTY``,
+  SIMP_TAC (srw_ss()) [FUN_EQ_THM, RIMAGE_DEF]);
+val _ = export_rewrites ["RIMAGE_REMPTY"]
+
 val imap_def = Define`
-  imap (f:'a action -> num) ((As,R):'a action_graph) =
-     (IMAGE (λa. a with iter := f a) As,
-      RIMAGE (λa. a with iter := f a) R)
+  imap (f:'a action -> num) (G: 'a action_graph) =
+     G with <| nodes updated_by IMAGE (λa. a with iter := f a);
+               edges updated_by RIMAGE (λa. a with iter := f a) |>
 `;
+
+val imap_emptyG = store_thm(
+  "imap_emptyG",
+  ``imap f emptyG = emptyG``,
+  simp[emptyG_def, imap_def]);
+val _ = export_rewrites ["imap_emptyG"]
+
+val IN_imap = store_thm(
+  "IN_imap",
+  ``a ∈ imap f G ⇔ ∃a0. a0 ∈ G ∧ a = a0 with iter := f a0``,
+  simp[imap_def] >> metis_tac[]);
+val _ = export_rewrites ["IN_imap"]
+
+val imap_edges = store_thm(
+  "imap_edges",
+  ``(imap f G).edges a1 a2 ⇔
+      ∃a10 a20. G.edges a10 a20 ∧ a1 = a10 with iter := f a10 ∧
+                a2 = a20 with iter := f a20``,
+  simp[imap_def, RIMAGE_DEF] >> metis_tac[]);
+
+val apply_action_ignores_iter = store_thm(
+  "apply_action_ignores_iter",
+  ``apply_action (a with iter updated_by f) A = apply_action a A``,
+  simp[apply_action_def]);
+val _ = export_rewrites ["apply_action_ignores_iter"]
 
 val imap_irrelevance = store_thm(
   "imap_irrelevance",
-  ``∀A0 AG A.
-      evalG A0 AG A ⇒
-      wfG AG ⇒
-        ∀f Is. INJ f (FST AG) Is ⇒ evalG A0 (imap f AG) A``,
-  Induct_on `evalG` >> simp[imap_def] >> rpt strip_tac >>
-  match_mp_tac (CONJUNCT2 evalG_rules) >> simp[RIMAGE_DEF] >>
-  `∀a1 a2. R a1 a2 ⇒ (a1 = a ∨ a1 ∈ as) ∧ (a2 = a ∨ a2 ∈ as)`
-     by metis_tac[wfG_def, IN_INSERT] >>
-  `∀a1 a2. (a1 = a ∨ a1 ∈ as) ∧ (a2 = a ∨ a2 ∈ as) ⇒
+  ``∀A0 G A.
+      evalG A0 G A ⇒
+      wfG G ⇒
+        ∀f Is. INJ f G.nodes Is ⇒ evalG A0 (imap f G) A``,
+  Induct_on `evalG` >> rpt strip_tac >> simp[] >>
+  match_mp_tac (CONJUNCT2 evalG_rules) >> dsimp[imap_edges] >>
+  qexists_tac `a` >> simp[] >> `wfG (G \\ a)` by simp[wfGs_pull_apart] >> fs[]>>
+  `∀a1 a2. a1 ∈ G ∧ a2 ∈ G ⇒
            (a1 with iter := f a1 = a2 with iter := f a2 ⇔
             a1 = a2)`
-    by (rpt gen_tac >> disch_then assume_tac >>
-        simp[Once (theorem "action_component_equality"), EQ_IMP_THM] >>
-        qpat_assum `INJ f XX YY` mp_tac >>
-        REWRITE_TAC[INJ_DEF, IN_INSERT] >> metis_tac[]) >>
-  rpt conj_tac >| [
-    dsimp[] >> map_every qx_gen_tac [`a1`, `a1'`, `a'`] >> strip_tac >>
-    Cases_on `R a1' a'` >> simp[] >>
-    Cases_on `a' = a`
-    >- (rw[] >> `a1' ∉ as` by metis_tac[] >> `a1' = a` by metis_tac[] >>
-        metis_tac[wfG_irrefl, IN_INSERT]) >>
-    `a' ∈ as` by metis_tac[] >> simp[],
-    qx_gen_tac `a2` >> Cases_on `a2 ∈ as` >> simp[] >> metis_tac[],
-    `apply_action (a with iter := f a) A0 = apply_action a A0`
-      by simp[apply_action_def] >> simp[] >>
-    `RIMAGE (λa. a with iter := f a) R \\ (a with iter := f a) =
-     RIMAGE (λa. a with iter := f a) (R \\ a)`
-      by (simp[FUN_EQ_THM, RIMAGE_DEF] >> metis_tac[]) >>
-    pop_assum SUBST1_TAC >> imp_res_tac wfGs_pull_apart >> fs[] >>
-    first_x_assum match_mp_tac >> qexists_tac `Is` >>
-    qpat_assum `INJ f XX YY` mp_tac >> metis_tac[INJ_INSERT]
-  ]);
+    by (rpt strip_tac >> fs[INJ_DEF] >> simp[EQ_IMP_THM] >>
+        simp[theorem "action_component_equality"]) >>
+  reverse conj_tac
+  >- (`imap f G \\ (a with iter := f a) = imap f (G \\ a)` suffices_by
+          (rw[] >> first_x_assum match_mp_tac >> fs[INJ_DEF] >> metis_tac[]) >>
+      dsimp[graph_equality, imap_edges, EQ_IMP_THM] >> csimp[] >>
+      rpt strip_tac
+      >- (pop_assum mp_tac >> `a10 ∈ G` by metis_tac[wfG_def] >> simp[] >>
+          metis_tac[]) >>
+      `a10 ∈ G` by metis_tac [wfG_def] >> metis_tac[]) >>
+  rpt gen_tac >>
+  qmatch_rename_tac `a0 ∈ G ⇒ ¬G.edges a1' a2' ∨ XX` ["XX"] >> strip_tac >>
+  Cases_on `G.edges a1' a2'` >> simp[] >>
+  `a1' ∈ G ∧ a2' ∈ G` by metis_tac[wfG_def] >> simp[] >> metis_tac[]);
 
 val example_t =
   ``FOR (0,N)
@@ -493,6 +535,25 @@ val vsub_eval_out_range_FOR = store_thm(
   qexists_tac `λj a. a ' i = A ' i` >> simp[eval_def] >>
   simp[update_sub]);
 
+val FOLDR_MAP_o = store_thm(
+  "FOLDR_MAP_o",
+  ``!l a. FOLDR f a (MAP g l) = FOLDR (f o g) a l``,
+  Induct THEN ASM_SIMP_TAC (srw_ss()) []);
+
+val FOLDL_MAP_combins = store_thm(
+  "FOLDL_MAP_combins",
+  ``!l a. FOLDL f a (MAP g l) = FOLDL (combin$C ((o) o f) g) a l``,
+  Induct THEN ASM_SIMP_TAC (srw_ss()) []);
+
+val mkEAction_o = store_thm(
+  "mkEAction_o",
+  ``mkEAction wf rfs body o f =
+    iter_fupd f o mkEAction (wf o f) (MAP (\rf. rf o f) rfs) (body o f)``,
+  simp[FUN_EQ_THM, mkEAction_def,
+       REWRITE_RULE [SINGL_DEF] SINGL_APPLY_PERMUTE,
+       REWRITE_RULE [SINGL_DEF] SINGL_APPLY_MAP, MAP_MAP_o,
+       combinTheory.o_ABS_R]);
+
 (* now convinced that this approach, based on what was done for
 "simple" loops, can't work because it's hard to imagine using it
 anything about the contents of the array part-way through the loop. In
@@ -550,6 +611,17 @@ Cases_on `i = n` >| [
       `δ n < N` by metis_tac[BIJ_DEF, IN_COUNT, SURJ_DEF] >>
       simp_tac (srw_ss())[eval_def]
 *)
+
+(*
+val FOLDR_example = prove(
+  ``BIJ f (count n) (count n) ⇒
+    FOLDR (INSERT) ∅ [0 ..< n] = FOLDR (INSERT) ∅ (MAP f [0 ..< n])``,
+  Induct_on `l` >> simp[] >> map_every qx_gen_tac [`h`, `m`] >>
+  Cases_on `MEM h l`
+  >- (`h INSERT set l = set l` by metis_tac[ABSORPTION] >>
+      simp[]
+*)
+
 
 (* val same_graphs = prove(
   ``(∀i0 i. ddepR wf rfs i0 i ==> δ i0 < δ i) ∧
